NatNormalForm/Equations.lean
@@ -1,0 +1,29 @@
+import NatNormalForm.Term
+
+
+theorem NatTerm.plus_zero_eq: forall {n: NatTerm}, (n + 0).Eq1 n := by
+  intros n
+  induction n with
+  | Z =>
+    apply NatTerm.R1.inclusion
+    apply NatTerm.R1.ZPlus
+  | S n' IHn' =>
+    apply NatTerm.Eq1.trans
+    . /- (n'.S + 0).Eq1 (n' + 0).S -/
+      apply NatTerm.R1.inclusion
+      apply NatTerm.R1.SPlus
+    . /- (n' + 0).S.Eq1 n'.S -/
+      apply NatTerm.Eq1.SCong
+      apply IHn'
+  | Plus n1 n2 IHn1 IHn2 =>
+    cases n1 with
+    | Z =>
+      have H: (Z.Plus n2 + 0).Eq1 (n2 + 0) := by
+        apply NatTerm.Eq1.PlusCong (.inclusion .ZPlus) .refl
+      apply NatTerm.Eq1.trans H
+      apply NatTerm.Eq1.trans IHn2
+      apply NatTerm.Eq1.symm (.inclusion .ZPlus)
+    | S m =>
+      admit
+    | _ => admit
+  | _ => admit
